Demo: progress in safety invariant; The problem is that we need to write lots of tedious proof

rustdemo/LinkedListSafe.v
@@ -37,26 +37,32 @@ Definition sound_cont (f: ident) : cont -> Prop :=
   else
     fun _ => False.
 
+Definition length_of_args (f: ident) : nat :=
+  if ident_eq f find then
+    2
+  else O.
+
 Inductive call_func (f: ident) : state -> Prop :=
-| call_func_intro: forall b ofs vl k m,
-    Genv.invert_symbol se b = Some f ->
+| call_func_intro: forall b vl k m
+    (SYM: Genv.invert_symbol se b = Some f)
     (** TODO: some property of k *)
-    sound_cont f k ->
-    call_func f (Callstate (Vptr b ofs) vl k m).
+    (SCONT: sound_cont f k)
+    (ARGS: length vl = length_of_args f),
+    call_func f (Callstate (Vptr b Ptrofs.zero) vl k m).
 
 (* continuation of the returnstate in find function *)
 Inductive find_cont_ret : cont -> Prop :=
-(* return the current find function *)
-| find_return1: forall k,
-    sound_find_cont k ->
-    find_cont_ret k
+(* (* return the current find function *) *)
+(* | find_return1: forall k, *)
+(*     sound_find_cont k -> *)
+(*     find_cont_ret k *)
 (* return from find *)
-| find_return2: forall k p f e own s,
+| find_return1: forall k p f e own s,
     sound_find_cont k ->
     (* TODO: specify the statement *)
     find_cont_ret (Kcall p f e own (Kseq s k))
 (* return from process *)
-| find_return3: forall k p f e own s,
+| find_return2: forall k p f e own s,
     sound_find_cont k ->
     (* TODO: specify the statement *)
     find_cont_ret (Kcall p f e own (Kseq s k))
@@ -68,5 +74,255 @@ Inductive return_find : state -> Prop :=
     find_cont_ret k ->
     return_find (Returnstate v k m).
 
+
+Fixpoint num_frames_cont (k: cont) : nat :=
+  match k with
+  | Kcall _ _ _ _ k' =>
+      S (num_frames_cont k')
+  | _ => O
+  end.
+
+Definition num_frames (s: state) : nat :=
+  match s with
+  | State _ _ k _ _ _
+  | Callstate _ _ k _
+  | Returnstate _ k _
+  | Dropinsert _ _ _ k _ _ _
+  | Dropplace _ _ _ k _ _ _
+  | Dropstate _ _ _ _ k _ => num_frames_cont k
+  end.
+              
+
 Inductive sound_state : state -> Prop :=
-| 
+| find_state_internal1: forall s0 s1 t n
+    (CALL: call_func find s0)
+    (STAR: starN step ge n s0 t s1)
+    (RAN: (0 <= n <= 3)%nat)
+    (* all execution is inside the current function *)
+    (NUMF: num_frames s0 = num_frames s1),
+    sound_state s1
+| find_state_internal2: forall s0 s1 t n,
+    return_find s0 ->
+    starN step ge n s0 t s1 ->
+    (0 <= n <= 3)%nat ->  
+    num_frames s0 = num_frames s1 ->
+    sound_state s1
+| find_returnstate: forall v k m,
+    sound_find_cont k ->
+    sound_state (Returnstate v k m).
+
+Lemma find_args_params_norepet:
+  list_norepet
+    (var_names (fn_params find_func) ++ var_names (fn_vars find_func)).
+Proof.
+  eapply proj_sumbool_true.
+  instantiate (1 := list_norepet_dec ident_eq (var_names (fn_params find_func) ++ var_names (fn_vars find_func))).
+  auto.
+Qed.
+
+
+Lemma init_own_env_find_progress:
+  exists own, init_own_env (Smallstep.globalenv (linked_list_sem se)) find_func = OK own.        
+  unfold init_own_env.
+  destruct collect_func eqn: A. cbn [bind].
+  set (empty_map := (PTree.map
+                       (fun (_ : positive) (_ : InitDomain.LPaths.t) =>
+                          InitDomain.Paths.empty) t)) in *.
+  set (initParams:= (InitDomain.add_place_list t
+                       (places_of_locals (fn_params find_func ++ fn_vars find_func))
+                       empty_map)) in *.
+  set (flag := check_own_env_consistency empty_map empty_map initParams t) in *.
+  generalize (eq_refl flag).             
+  generalize flag at 1 3.
+  intros flag0 E. destruct flag0; try congruence.
+  eexists; eauto.
+  unfold flag in E. unfold initParams, empty_map in *.
+  unfold collect_func in A.
+  replace t with ((collect_stmt (Smallstep.globalenv (linked_list_sem se))
+           (fn_body find_func)
+           (fold_right
+              (InitDomain.collect_place
+                 (Smallstep.globalenv (linked_list_sem se)))
+              (PTree.empty InitDomain.LPaths.t)
+              (map
+                 (fun elt : ident * type => Plocal (fst elt) (snd elt))
+                 (fn_params find_func ++ fn_vars find_func))))) in *.
+  change (check_own_env_consistency
+        (PTree.map
+           (fun (_ : positive) (_ : InitDomain.LPaths.t) =>
+            InitDomain.Paths.empty)
+           (collect_stmt (Smallstep.globalenv (linked_list_sem se))
+              (fn_body find_func)
+              (fold_right
+                 (InitDomain.collect_place
+                    (Smallstep.globalenv (linked_list_sem se)))
+                 (PTree.empty InitDomain.LPaths.t)
+                 (map
+                    (fun elt : ident * type =>
+                     Plocal (fst elt) (snd elt))
+                    (fn_params find_func ++ fn_vars find_func)))))
+        (PTree.map
+           (fun (_ : positive) (_ : InitDomain.LPaths.t) =>
+            InitDomain.Paths.empty)
+           (collect_stmt (Smallstep.globalenv (linked_list_sem se))
+              (fn_body find_func)
+              (fold_right
+                 (InitDomain.collect_place
+                    (Smallstep.globalenv (linked_list_sem se)))
+                 (PTree.empty InitDomain.LPaths.t)
+                 (map
+                    (fun elt : ident * type =>
+                     Plocal (fst elt) (snd elt))
+                    (fn_params find_func ++ fn_vars find_func)))))
+        (InitDomain.add_place_list
+           (collect_stmt (Smallstep.globalenv (linked_list_sem se))
+              (fn_body find_func)
+              (fold_right
+                 (InitDomain.collect_place
+                    (Smallstep.globalenv (linked_list_sem se)))
+                 (PTree.empty InitDomain.LPaths.t)
+                 (map
+                    (fun elt : ident * type =>
+                     Plocal (fst elt) (snd elt))
+                    (fn_params find_func ++ fn_vars find_func))))
+           (places_of_locals (fn_params find_func ++ fn_vars find_func))
+           (PTree.map
+              (fun (_ : positive) (_ : InitDomain.LPaths.t) =>
+               InitDomain.Paths.empty)
+              (collect_stmt (Smallstep.globalenv (linked_list_sem se))
+                 (fn_body find_func)
+                 (fold_right
+                    (InitDomain.collect_place
+                       (Smallstep.globalenv (linked_list_sem se)))
+                    (PTree.empty InitDomain.LPaths.t)
+                    (map
+                       (fun elt : ident * type =>
+                        Plocal (fst elt) (snd elt))
+                       (fn_params find_func ++ fn_vars find_func))))))
+        (collect_stmt (Smallstep.globalenv (linked_list_sem se))
+           (fn_body find_func)
+           (fold_right
+              (InitDomain.collect_place
+                 (Smallstep.globalenv (linked_list_sem se)))
+              (PTree.empty InitDomain.LPaths.t)
+              (map
+                 (fun elt : ident * type => Plocal (fst elt) (snd elt))
+                 (fn_params find_func ++ fn_vars find_func))))) with true in *. congruence.
+  (* reflexivity. *)
+  congruence.
+  unfold collect_func in A. congruence.
+Qed.
+                                                                                
+Lemma step_preservation_progress: forall s,
+    sound_state s ->
+    (not_stuck (linked_list_sem se) s \/ step_mem_error ge s)
+    /\ (forall s' t, step ge s t s' ->
+               sound_state s').
+Proof.
+  intros s INV. inv INV.
+  - generalize CALL as CALL1.
+    generalize STAR as STAR1. intros.
+    (* build s0 *)
+    inv CALL.
+    assert (FIND: Genv.find_funct ge (Vptr b Ptrofs.zero) = Some (Internal find_func)).
+    { simpl. destruct Ptrofs.eq_dec; try congruence.
+      eapply Genv.find_funct_ptr_iff.
+      rewrite Genv.find_def_spec. rewrite SYM.
+      auto. }
+    inv STAR.
+    (* take zero step *)
+    { split.
+      - left. red. right. right.
+        do 2 eexists.
+        econstructor; eauto.
+        
+
+        Lemma init_own_env_find_progress:
+          exists own, init_own_env (Smallstep.globalenv (linked_list_sem se)) find_func =
+ OK own.
+        
+        2: { unfold init_own_env.
+             destruct collect_func eqn: A. cbn [bind].
+             set (empty_map := (PTree.map
+         (fun (_ : positive) (_ : InitDomain.LPaths.t) =>
+            InitDomain.Paths.empty) t)) in *.
+             set (initParams:= (InitDomain.add_place_list t
+         (places_of_locals (fn_params find_func ++ fn_vars find_func))
+         empty_map)) in *.
+             set (flag := check_own_env_consistency empty_map empty_map initParams t) in *.
+             generalize (eq_refl flag).             
+             generalize flag at 1 3.
+             intros flag0 E. destruct flag0; try congruence.
+             
+             generalize (check_own_env_consistency
+       (PTree.map
+          (fun (_ : positive) (_ : InitDomain.LPaths.t) =>
+           InitDomain.Paths.empty) t)
+       (PTree.map
+          (fun (_ : positive) (_ : InitDomain.LPaths.t) =>
+           InitDomain.Paths.empty) t)
+       (InitDomain.add_place_list t
+          (places_of_locals (fn_params find_func ++ fn_vars find_func))
+          (PTree.map
+             (fun (_ : positive) (_ : InitDomain.LPaths.t) =>
+              InitDomain.Paths.empty) t))) at 1,3 .
+
+             
+             replace (check_own_env_consistency
+      (PTree.map
+         (fun (_ : positive) (_ : InitDomain.LPaths.t) =>
+          InitDomain.Paths.empty)
+         (collect_func (Smallstep.globalenv (linked_list_sem se))
+            find_func))
+      (PTree.map
+         (fun (_ : positive) (_ : InitDomain.LPaths.t) =>
+          InitDomain.Paths.empty)
+         (collect_func (Smallstep.globalenv (linked_list_sem se))
+            find_func))
+      (InitDomain.add_place_list
+         (collect_func (Smallstep.globalenv (linked_list_sem se))
+            find_func)
+         (places_of_locals (fn_params find_func ++ fn_vars find_func))
+         (PTree.map
+            (fun (_ : positive) (_ : InitDomain.LPaths.t) =>
+             InitDomain.Paths.empty)
+            (collect_func (Smallstep.globalenv (linked_list_sem se))
+               find_func)))
+      (collect_func (Smallstep.globalenv (linked_list_sem se))
+         find_func)) with true.
+
+
+native_compute (check_own_env_consistency
+      (PTree.map
+         (fun (_ : positive) (_ : InitDomain.LPaths.t) =>
+          InitDomain.Paths.empty)
+         (collect_func (proj1_sig build_ce_ok) find_func))
+      (PTree.map
+         (fun (_ : positive) (_ : InitDomain.LPaths.t) =>
+          InitDomain.Paths.empty)
+         (collect_func (proj1_sig build_ce_ok) find_func))
+      (InitDomain.add_place_list
+         (collect_func (proj1_sig build_ce_ok) find_func)
+         (places_of_locals (fn_params find_func ++ fn_vars find_func))
+         (PTree.map
+            (fun (_ : positive) (_ : InitDomain.LPaths.t) =>
+             InitDomain.Paths.empty)
+            (collect_func (proj1_sig build_ce_ok) find_func)))
+      (collect_func (proj1_sig build_ce_ok) find_func) = true).
+{ simpl
+
+
+    
+  rewrite H.
+             
+               
+        econstructor.
+        eapply find_args_params_norepet.
+        eapply do_alloc_variables_sound. simpl.
+        do 9 destruct Mem.alloc eqn: ?ALLOC at 1. f_equal.
+
+        Lemma find_step_internal_progress
+
+
+        
+                
